Fix internalize, guarded

theories/Misc/Guarded.v
@@ -10,6 +10,303 @@ From CTree Require Import
 
 Import MonadNotation.
 Open Scope monad_scope.
+
+Definition guarded_form {E B X} `{B1 -< B} (t : ctree E B X) : ctree E B X :=
+  CTree.iter (fun t =>
+				        match observe t with
+				        | RetF r => ret (inr r)
+				        | BrDF n k => BrD n (fun x => ret (inl (k x)))
+				        | BrSF n k => BrD n (fun x => Step (ret (inl (k x))))
+				        | VisF e k => bind (mtrigger e) (fun x => ret (inl (k x)))
+				        end) t.
+
+(* TODO move *)
+Arguments MonadTrigger_ctree /.
+
+Lemma unfold_guarded_form {E B X} `{B1 -< B} (t : ctree E B X) :
+  guarded_form t ≅
+  match observe t with
+	| RetF r => ret r
+  | BrDF n k =>
+      BrD n (fun x => Guard (guarded_form (k x)))
+	| BrSF n k =>
+      BrD n (fun x => Step (Guard (guarded_form (k x))))
+	| VisF e k => bind (mtrigger e) (fun x => Guard (guarded_form (k x)))
+	end.
+Proof.
+  unfold guarded_form at 1.
+  rewrite unfold_iter.
+  desobs t; cbn.
+  - now rewrite bind_ret_l.
+  - unfold mtrigger; cbn.
+    rewrite bind_bind, !bind_trigger.
+    step; constructor; intros ?.
+    rewrite bind_ret_l.
+    reflexivity.
+  - destruct vis.
+    + rewrite bind_br.
+      step; constructor; intros ?.
+      rewrite bind_step; step; constructor; intros ?.
+      rewrite bind_ret_l.
+      step; constructor; auto.
+    + rewrite bind_br.
+      step; constructor; intros ?.
+      rewrite bind_ret_l.
+      step; constructor; auto.
+Qed.
+
+Lemma trans_guarded_inv_strong :
+  forall {E B X} `{HasStuck : B0 -< B} `{HasTau : B1 -< B} (t u v : ctree E B X) l,
+    (v ≅ guarded_form t \/ v ≅ Guard (guarded_form t)) ->
+    trans l v u ->
+    exists t', trans l t t'
+          /\ (u ≅ guarded_form t' \/ u ≅ Guard (guarded_form t')).
+Proof.
+  intros * EQ TR.
+  revert t EQ.
+  unfold trans in TR; repeat red in TR.
+  dependent induction TR.
+  - intros ? [EQ | EQ].
+    + rewrite ctree_eta, <- x, unfold_guarded_form in EQ.
+      setoid_rewrite (ctree_eta t).
+      desobs t; try now step in EQ; inv EQ.
+      destruct vis.
+      * pose proof equ_br_invT _ _ _ _ EQ as [<- _].
+        apply equ_br_invE with (x := x0) in EQ .
+        rewrite EQ in TR.
+        apply trans_step_inv in TR as [EQ' ->].
+        eexists; split; eauto.
+        etrans.
+      * pose proof equ_br_invT _ _ _ _ EQ as [<- _].
+        apply equ_br_invE with (x := x0) in EQ .
+        specialize (IHTR _ _ eq_refl eq_refl).
+        edestruct IHTR as (t' & ? & ?); eauto.
+        exists t'.
+        split.
+        eapply trans_brD with (x := x0); eauto.
+        eauto.
+
+    + rewrite ctree_eta, <- x in EQ.
+      pose proof equ_br_invT _ _ _ _ EQ as [-> _].
+      apply equ_br_invE with (x := x0) in EQ .
+      specialize (IHTR _ _ eq_refl eq_refl).
+      edestruct IHTR as (t' & ? & ?); eauto.
+
+  - (* G(t) ≅ BrS k : absurd *)
+    intros ? [EQ | EQ].
+    + rewrite ctree_eta, <- x1, unfold_guarded_form in EQ.
+      desobs t0; try now step in EQ; inv EQ.
+      destruct vis; try now step in EQ; inv EQ.
+    + rewrite ctree_eta, <- x1 in EQ.
+      now step in EQ; inv EQ.
+
+  - (* G(t) ≅ Vis e k : t ≅ Vis e k', k x ≅ Guard (G (k' x)) *)
+    intros ? [EQ | EQ].
+    + setoid_rewrite (ctree_eta t0).
+      rewrite ctree_eta, <- x1, unfold_guarded_form in EQ.
+      rewrite (ctree_eta t), x in H.
+      clear t x.
+      desobs t0; try now step in EQ; inv EQ.
+      2:destruct vis; try now step in EQ; inv EQ.
+      cbn in *.
+      unfold mtrigger in EQ; rewrite bind_trigger in EQ.
+      pose proof equ_vis_invT _ _ _ _ EQ; subst.
+      pose proof equ_vis_invE _ _ _ _ EQ as [-> EQ'].
+      eexists; split.
+      etrans.
+      rewrite <- ctree_eta in H.
+      rewrite <- H.
+      rewrite EQ'.
+      auto.
+    + rewrite ctree_eta, <- x1 in EQ.
+      now step in EQ; inv EQ.
+
+  - (* G(t) ≅ Ret x : t ≅ Ret x *)
+    intros ? [EQ | EQ].
+    + setoid_rewrite (ctree_eta t).
+      rewrite ctree_eta, <- x0, unfold_guarded_form in EQ.
+      desobs t; try now step in EQ; inv EQ.
+      2:destruct vis; try now step in EQ; inv EQ.
+      step in EQ; inv EQ.
+      eexists; split.
+      etrans.
+      left.
+      rewrite ctree_eta, <- x, unfold_guarded_form.
+      cbn.
+      rewrite ! brD0_always_stuck.
+      reflexivity.
+    + rewrite ctree_eta, <- x0 in EQ.
+      now step in EQ; inv EQ.
+Qed.
+
+Lemma trans_guarded_inv :
+  forall E B X `(B0 -< B) `(B1 -< B) (t u : ctree E B X) l,
+    trans l (guarded_form t) u ->
+    exists t', trans l t t'
+          /\ u ~ guarded_form t'.
+Proof.
+  intros.
+  edestruct @trans_guarded_inv_strong as (t' & TR & EQ); [|eassumption|].
+  left; eauto.
+  exists t'; split; auto.
+  destruct EQ as [EQ |EQ]; rewrite EQ; auto.
+  rewrite sb_guard; auto.
+Qed.
+
+#[global] Instance guarded_equ E B X `(B1 -< B) : Proper (equ eq ==> equ eq) (@guarded_form E B X _).
+Proof.
+  do 2 red.
+  coinduction ? IH.
+  intros * EQ.
+  step in EQ.
+  rewrite ! unfold_guarded_form.
+  cbn*.
+  inv EQ; auto.
+  - cbn.
+    constructor; intros ?.
+    fold_subst; rewrite ! bind_ret_l.
+    step; constructor; intros _.
+    auto.
+  - destruct b; cbn.
+    all: constructor; intros ?.
+    all: repeat (step; constructor; intros ?).
+    all: auto.
+Qed.
+
+(* TODO: bind simpl never globally? *)
+(* TODO: Taus without continuation? *)
+(* TODO: tactic for better stepping for equ *)
+(* TODO: tactics for better stepping for sbisim (see a couple above) *)
+(* Equality on [observe u] rewritten in [equ]? *)
+Opaque CTree.bind.
+Lemma trans_guarded_strong :
+  forall E B X `(HasStuck : B0 -< B) `(HasTau : B1 -< B) (t u : ctree E B X) l,
+    trans l t u ->
+    exists u',
+      trans l (guarded_form t) u'
+      /\ (u' ≅ guarded_form u
+         \/ u' ≅ Guard (guarded_form u)).
+Proof.
+  intros * TR.
+  (* revert t EQ. *)
+  unfold trans in TR; repeat red in TR.
+  dependent induction TR; intros.
+  - (* destruct EQ as [EQ | EQ]. *)
+    edestruct IHTR as (u' & TR' & EQ'); eauto.
+    setoid_rewrite unfold_guarded_form at 1; rewrite <- x.
+    exists u'; split.
+    eapply trans_brD with (x := x0); [| reflexivity].
+    now apply trans_guard.
+    auto.
+  - setoid_rewrite unfold_guarded_form at 1; rewrite <- x1.
+    eexists; split.
+    eapply trans_brD with (x := x0); [| reflexivity].
+    etrans.
+    right.
+    step; constructor; intros ?.
+    rewrite H.
+    rewrite (ctree_eta t0),x,<- ctree_eta.
+    auto.
+  - setoid_rewrite unfold_guarded_form at 1; rewrite <- x1.
+    eexists; split.
+    unfold mtrigger, MonadTrigger_ctree; cbn.
+    rewrite bind_trigger.
+    etrans.
+    right.
+    step; constructor; intros ?.
+    rewrite H.
+    rewrite (ctree_eta t0),x,<- ctree_eta.
+    auto.
+  - setoid_rewrite unfold_guarded_form at 1; rewrite <- x0.
+    eexists; split.
+    (*
+      Why do I need to cbn even if I add:
+      Hint Unfold ret Monad_ctree : trans.
+     *)
+    cbn; etrans.
+    left.
+    rewrite unfold_guarded_form, <- x; cbn.
+    now rewrite ! brD0_always_stuck.
+Qed.
+
+Lemma trans_guarded :
+  forall E B X `(B0 -< B) `(B1 -< B) (t u : ctree E B X) l,
+    trans l t u ->
+    exists u',
+      trans l (guarded_form t) u'
+      /\ u' ~ guarded_form u.
+Proof.
+  intros * TR.
+  edestruct trans_guarded_strong as (u' & TR' & EQ'); eauto.
+  exists u'; split; eauto.
+  destruct EQ' as [EQ' | EQ']; rewrite EQ'; auto.
+  now rewrite sb_guard.
+Qed.
+
+(* TODO: define properly the set of tactics in [sbisim] and kill this.
+   TODO: this is not resilient enough, it loops if the goal is not exactly of the right shape
+ *)
+Ltac sret  := apply step_sb_ret.
+Ltac svis  := apply step_sb_vis_id || apply step_sb_vis.
+Ltac sStep := apply step_sb_step.
+Ltac sstep := sret || svis || sStep.
+
+Lemma guarded_is_bisimilar {E B X} `{B0 -< B} `{B1 -< B} : forall (t : ctree E B X),
+    guarded_form t ~ t.
+Proof.
+  coinduction ? IH.
+  intros t.
+  rewrite (ctree_eta t) at 2.
+  rewrite unfold_guarded_form.
+  desobs t.
+  - now cbn.
+  - cbn.
+    unfold mtrigger; rewrite bind_trigger.
+    svis; intros ?.
+    rewrite sb_guard.
+    apply IH.
+    reflexivity.
+  - destruct vis.
+    + cbn.
+      split; intros ? ? TR.
+      * inv_trans.
+        subst.
+        do 2 eexists.
+        split; [etrans |].
+        split; [| reflexivity].
+        rewrite EQ.
+        rewrite sb_guard.
+        apply IH.
+      * cbn.
+        inv_trans; subst.
+        do 2 eexists.
+        split; [etrans |].
+        split; [| reflexivity ].
+        rewrite sb_guard.
+        rewrite EQ; apply IH.
+    + split.
+      * intros ? ? TR.
+        cbn.
+        inv_trans.
+        edestruct trans_guarded_inv as (u' & TR' & EQ'); eauto.
+        do 2 eexists.
+        split; [etrans |].
+        split; [| reflexivity].
+        rewrite EQ'; auto.
+      * cbn; intros ? ? TR.
+        inv_trans.
+        edestruct trans_guarded as (u' & TR' & EQ'); eauto.
+        do 2 eexists.
+        split; [etrans |].
+        split; [| reflexivity].
+        rewrite EQ'; auto.
+Qed.
+
+
+(* TODO MOVE AND FIX THIS
+
+
+
 <<<<<<< HEAD:theories/Interp/Sched.v
 
 #[global] Instance ctree_trigger {E C} : MonadTrigger E (ctree E C) :=
@@ -317,379 +614,4 @@ Prove that the original computation simulates the scheduled one?
 *)
 
 
-Definition guarded_form {E C X} `{C1 -< C} (t : ctree E C X) : ctree E C X :=
-	CTree.iter (fun t =>
-				        match observe t with
-				        | RetF r => ret (inr r)
-				        | ChoiceIF c k =>
-                    ChoiceI c (fun x => Ret (inl (k x)))
-				        | ChoiceVF c k =>
-                    ChoiceI c (fun x => tauV (Ret (inl (k x))))
-				        | VisF e k => bind (mtrigger _ e) (fun x => Ret (inl (k x)))
-=======
-Notation BrSF := (BrF true).
-Notation BrDF := (BrF false).
-
-Definition guarded_form {E X} (t : ctree E X) : ctree E X :=
-	CTree.iter (fun t =>
-				        match observe t with
-				        | RetF r => ret (inr r)
-				        | BrDF n k =>
-                    BrD n (fun x => ret (inl (k x)))
-				        | BrSF n k =>
-                    BrD n (fun x => Step (ret (inl (k x))))
-				        | VisF e k => bind (mtrigger _ e) (fun x => ret (inl (k x)))
->>>>>>> master:theories/Misc/Guarded.v
-				        end) t.
-
-Lemma unfold_guarded_form {E C X} `{C1 -< C} (t : ctree E C X) :
-  guarded_form t ≅
-  match observe t with
-	| RetF r => ret r
-<<<<<<< HEAD:theories/Interp/Sched.v
-	| ChoiceIF c k =>
-      ChoiceI c (fun x => tauI (guarded_form (k x)))
-	| ChoiceVF c k =>
-      ChoiceI c (fun x => tauV (tauI (guarded_form (k x))))
-	| VisF e k => bind (mtrigger _ e) (fun x => tauI (guarded_form (k x)))
-=======
-	| BrDF n k =>
-      BrD n (fun x => Guard (guarded_form (k x)))
-	| BrSF n k =>
-      BrD n (fun x => Step (Guard (guarded_form (k x))))
-	| VisF e k => bind (mtrigger _ e) (fun x => Guard (guarded_form (k x)))
->>>>>>> master:theories/Misc/Guarded.v
-	end.
-Proof.
-  unfold guarded_form at 1.
-  rewrite unfold_iter.
-  desobs t; cbn.
-  - now rewrite bind_ret_l.
-  - unfold mtrigger; rewrite bind_bind, !bind_trigger.
-    step; constructor; intros ?.
-    rewrite bind_ret_l.
-    reflexivity.
-  - destruct vis.
-    + rewrite bind_br.
-      step; constructor; intros ?.
-      rewrite bind_Step; step; constructor; intros ?.
-      rewrite bind_ret_l.
-      step; constructor; auto.
-    + rewrite bind_br.
-      step; constructor; intros ?.
-      rewrite bind_ret_l.
-      step; constructor; auto.
-Qed.
-
-Lemma trans_guarded_inv_strong :
-<<<<<<< HEAD:theories/Interp/Sched.v
-  forall {E C X} `{HasStuck : C0 -< C} `{HasTau : C1 -< C} (t u v : ctree E C X) l,
-    (v ≅ guarded_form t \/ v ≅ tauI (guarded_form t)) ->
-    trans l v u ->
-    exists t', trans l t t'
-          /\ (u ≅ guarded_form t' \/ u ≅ tauI (guarded_form t')).
-=======
-  forall {E X} (t u v : ctree E X) l,
-    (v ≅ guarded_form t \/ v ≅ Guard (guarded_form t)) ->
-    trans l v u ->
-    exists t', trans l t t'
-          /\ (u ≅ guarded_form t' \/ u ≅ Guard (guarded_form t')).
->>>>>>> master:theories/Misc/Guarded.v
-Proof.
-  intros * EQ TR.
-  revert t EQ.
-  unfold trans in TR; repeat red in TR.
-  dependent induction TR.
-  - intros ? [EQ | EQ].
-    + rewrite ctree_eta, <- x, unfold_guarded_form in EQ.
-      setoid_rewrite (ctree_eta t).
-      desobs t; try now step in EQ; inv EQ.
-      destruct vis.
-<<<<<<< HEAD:theories/Interp/Sched.v
-      * pose proof equ_choice_invT _ _ _ _ EQ as [<- _].
-        apply equ_choice_invE with (x := x0) in EQ .
-=======
-      * pose proof equ_br_invT _ _ EQ as [<- _].
-        apply equ_br_invE with (x := x0) in EQ .
->>>>>>> master:theories/Misc/Guarded.v
-        rewrite EQ in TR.
-        apply trans_step_inv in TR as [EQ' ->].
-        eexists; split; eauto.
-        etrans.
-
-<<<<<<< HEAD:theories/Interp/Sched.v
-      * pose proof equ_choice_invT _ _ _ _ EQ as [<- _].
-        apply equ_choice_invE with (x := x0) in EQ .
-=======
-      * pose proof equ_br_invT _ _ EQ as [<- _].
-        apply equ_br_invE with (x := x0) in EQ .
->>>>>>> master:theories/Misc/Guarded.v
-        specialize (IHTR _ _ eq_refl eq_refl).
-        edestruct IHTR as (t' & ? & ?); eauto.
-        exists t'.
-        split.
-        eapply trans_brD with (x := x0); eauto.
-        eauto.
-
-    + rewrite ctree_eta, <- x in EQ.
-<<<<<<< HEAD:theories/Interp/Sched.v
-      pose proof equ_choice_invT _ _ _ _ EQ as [-> _].
-      apply equ_choice_invE with (x := x0) in EQ .
-=======
-      pose proof equ_br_invT _ _ EQ as [-> _].
-      apply equ_br_invE with (x := x0) in EQ .
->>>>>>> master:theories/Misc/Guarded.v
-      specialize (IHTR _ _ eq_refl eq_refl).
-      edestruct IHTR as (t' & ? & ?); eauto.
-
-  - (* G(t) ≅ BrS k : absurd *)
-    intros ? [EQ | EQ].
-    + rewrite ctree_eta, <- x1, unfold_guarded_form in EQ.
-      desobs t0; try now step in EQ; inv EQ.
-      destruct vis; try now step in EQ; inv EQ.
-    + rewrite ctree_eta, <- x1 in EQ.
-      now step in EQ; inv EQ.
-
-  - (* G(t) ≅ Vis e k : t ≅ Vis e k', k x ≅ Guard (G (k' x)) *)
-    intros ? [EQ | EQ].
-    + setoid_rewrite (ctree_eta t0).
-      rewrite ctree_eta, <- x1, unfold_guarded_form in EQ.
-      rewrite (ctree_eta t), x in H.
-      clear t x.
-      desobs t0; try now step in EQ; inv EQ.
-      2:destruct vis; try now step in EQ; inv EQ.
-      cbn in *.
-      unfold mtrigger in EQ; rewrite bind_trigger in EQ.
-      pose proof equ_vis_invT _ _ _ _ EQ; subst.
-      pose proof equ_vis_invE _ _ _ _ EQ as [-> EQ'].
-      eexists; split.
-      etrans.
-      rewrite <- ctree_eta in H.
-      rewrite <- H.
-      rewrite EQ'.
-      auto.
-    + rewrite ctree_eta, <- x1 in EQ.
-      now step in EQ; inv EQ.
-
-  - (* G(t) ≅ Ret x : t ≅ Ret x *)
-    intros ? [EQ | EQ].
-    + setoid_rewrite (ctree_eta t).
-      rewrite ctree_eta, <- x0, unfold_guarded_form in EQ.
-      desobs t; try now step in EQ; inv EQ.
-      2:destruct vis; try now step in EQ; inv EQ.
-      step in EQ; inv EQ.
-      eexists; split.
-      etrans.
-      left.
-      rewrite ctree_eta, <- x, unfold_guarded_form.
-      cbn.
-<<<<<<< HEAD:theories/Interp/Sched.v
-      rewrite ! choice0_always_stuck.
-=======
-      rewrite ! brD0_always_stuck.
->>>>>>> master:theories/Misc/Guarded.v
-      reflexivity.
-    + rewrite ctree_eta, <- x0 in EQ.
-      now step in EQ; inv EQ.
-Qed.
-
-Lemma trans_guarded_inv :
-  forall E C X `(C0 -< C) `(C1 -< C) (t u : ctree E C X) l,
-    trans l (guarded_form t) u ->
-    exists t', trans l t t'
-          /\ u ~ guarded_form t'.
-Proof.
-  intros.
-  edestruct @trans_guarded_inv_strong as (t' & TR & EQ); [|eassumption|].
-  left; eauto.
-  exists t'; split; auto.
-  destruct EQ as [EQ |EQ]; rewrite EQ; auto.
-  rewrite sb_guard; auto.
-Qed.
-
-#[global] Instance guarded_equ E C X `(C1 -< C) : Proper (equ eq ==> equ eq) (@guarded_form E C X _).
-Proof.
-  do 2 red.
-  coinduction ? IH.
-  intros * EQ.
-  step in EQ.
-  rewrite ! unfold_guarded_form.
-  cbn*.
-  inv EQ; auto.
-  - cbn.
-    constructor; intros ?.
-    fold_subst; rewrite ! bind_ret_l.
-    step; constructor; intros _.
-    auto.
-  - destruct b; cbn.
-    all: constructor; intros ?.
-    all: repeat (step; constructor; intros ?).
-    all: auto.
-Qed.
-
-(* TODO: bind simpl never globally? *)
-(* TODO: Taus without continuation? *)
-(* TODO: tactic for better stepping for equ *)
-(* TODO: tactics for better stepping for sbisim (see a couple above) *)
-(* Equality on [observe u] rewritten in [equ]? *)
-Opaque CTree.bind.
-Lemma trans_guarded_strong :
-  forall E C X `(HasStuck : C0 -< C) `(HasTau : C1 -< C) (t u : ctree E C X) l,
-    trans l t u ->
-    exists u',
-      trans l (guarded_form t) u'
-      /\ (u' ≅ guarded_form u
-<<<<<<< HEAD:theories/Interp/Sched.v
-         \/ u' ≅ tauI (guarded_form u)).
-=======
-         \/ u' ≅ Guard (guarded_form u)).
->>>>>>> master:theories/Misc/Guarded.v
-Proof.
-  intros * TR.
-  (* revert t EQ. *)
-  unfold trans in TR; repeat red in TR.
-  dependent induction TR; intros.
-  - (* destruct EQ as [EQ | EQ]. *)
-    edestruct IHTR as (u' & TR' & EQ'); eauto.
-    setoid_rewrite unfold_guarded_form at 1; rewrite <- x.
-    exists u'; split.
-    eapply trans_brD with (x := x0); [| reflexivity].
-    now apply trans_guard.
-    auto.
-  - setoid_rewrite unfold_guarded_form at 1; rewrite <- x1.
-    eexists; split.
-    eapply trans_brD with (x := x0); [| reflexivity].
-    etrans.
-    right.
-    step; constructor; intros ?.
-    rewrite H.
-    rewrite (ctree_eta t0),x,<- ctree_eta.
-    auto.
-  - setoid_rewrite unfold_guarded_form at 1; rewrite <- x1.
-    eexists; split.
-    unfold mtrigger, MonadTrigger_ctree; cbn.
-    rewrite bind_trigger.
-    etrans.
-    right.
-    step; constructor; intros ?.
-    rewrite H.
-    rewrite (ctree_eta t0),x,<- ctree_eta.
-    auto.
-  - setoid_rewrite unfold_guarded_form at 1; rewrite <- x0.
-    eexists; split.
-    (*
-      Why do I need to cbn even if I add:
-      Hint Unfold ret Monad_ctree : trans.
-     *)
-    cbn; etrans.
-    left.
-    rewrite unfold_guarded_form, <- x; cbn.
-<<<<<<< HEAD:theories/Interp/Sched.v
-    now rewrite ! choice0_always_stuck.
-=======
-    now rewrite ! brD0_always_stuck.
->>>>>>> master:theories/Misc/Guarded.v
-Qed.
-
-Lemma trans_guarded :
-  forall E C X `(C0 -< C) `(C1 -< C) (t u : ctree E C X) l,
-    trans l t u ->
-    exists u',
-      trans l (guarded_form t) u'
-      /\ u' ~ guarded_form u.
-Proof.
-  intros * TR.
-  edestruct trans_guarded_strong as (u' & TR' & EQ'); eauto.
-  exists u'; split; eauto.
-  destruct EQ' as [EQ' | EQ']; rewrite EQ'; auto.
-  now rewrite sb_guard.
-Qed.
-
-(* TODO: define properly the set of tactics in [sbisim] and kill this.
-   TODO: this is not resilient enough, it loops if the goal is not exactly of the right shape
  *)
-Ltac sret  := apply step_sb_ret.
-Ltac svis  := apply step_sb_vis.
-Ltac sStep := apply step_sb_step.
-Ltac sstep := sret || svis || sStep.
-
-Lemma guarded_is_bisimilar {E C X} `{C0 -< C} `{C1 -< C} : forall (t : ctree E C X),
-    guarded_form t ~ t.
-Proof.
-  coinduction ? IH.
-  intros t.
-  rewrite (ctree_eta t) at 2.
-  rewrite unfold_guarded_form.
-  desobs t.
-  - now cbn.
-  - cbn.
-    unfold mtrigger; rewrite bind_trigger.
-<<<<<<< HEAD:theories/Interp/Sched.v
-    svis; intros ?.
-    rewrite sb_tauI.
-=======
-    sstep; intros ?.
-    rewrite sb_guard.
->>>>>>> master:theories/Misc/Guarded.v
-    apply IH.
-  - destruct vis.
-    + cbn.
-      split; intros ? ? TR.
-      * inv_trans.
-        subst.
-<<<<<<< HEAD:theories/Interp/Sched.v
-        eexists. eexists.
-        split; [etrans |].
-        split; [| reflexivity].
-=======
-        eexists.
-        eapply trans_brS with (x := x).
->>>>>>> master:theories/Misc/Guarded.v
-        rewrite EQ.
-        rewrite sb_guard.
-        apply IH.
-      * cbn.
-        inv_trans; subst.
-<<<<<<< HEAD:theories/Interp/Sched.v
-        eexists. eexists.
-        split; [etrans |].
-        split; [| reflexivity ].
-        rewrite sb_tauI.
-=======
-        eexists.
-        eapply trans_brD with (x := x).
-        2:etrans.
-        etrans.
-        rewrite sb_guard.
->>>>>>> master:theories/Misc/Guarded.v
-        rewrite EQ; apply IH.
-    + split.
-      * intros ? ? TR.
-        cbn.
-        inv_trans.
-        edestruct trans_guarded_inv as (u' & TR' & EQ'); eauto.
-<<<<<<< HEAD:theories/Interp/Sched.v
-        eexists. eexists.
-        split; [etrans |].
-        split; [| reflexivity].
-=======
-        eexists.
-        eapply trans_brD with (x := x); [| reflexivity].
-        eassumption.
->>>>>>> master:theories/Misc/Guarded.v
-        rewrite EQ'; auto.
-      * cbn; intros ? ? TR.
-        inv_trans.
-        edestruct trans_guarded as (u' & TR' & EQ'); eauto.
-<<<<<<< HEAD:theories/Interp/Sched.v
-        eexists. eexists.
-        split; [etrans |].
-        split; [| reflexivity].
-=======
-        eexists.
-        eapply trans_brD with (x := x); [| reflexivity].
-        apply trans_guard.
-        eauto.
->>>>>>> master:theories/Misc/Guarded.v
-        rewrite EQ'; auto.
-Qed.
